asllib/acl2/manual.lisp
@@ -1,0 +1,55 @@
+;;****************************************************************************;;
+;;                                ASLRef                                      ;;
+;;****************************************************************************;;
+;;
+;; SPDX-FileCopyrightText: Copyright 2025 Arm Limited and/or its affiliates <open-source-office@arm.com>
+;; SPDX-License-Identifier: BSD-3-Clause
+;; 
+;;****************************************************************************;;
+;; Disclaimer:                                                                ;;
+;; This material covers both ASLv0 (viz, the existing ASL pseudocode language ;;
+;; which appears in the Arm Architecture Reference Manual) and ASLv1, a new,  ;;
+;; experimental, and as yet unreleased version of ASL.                        ;;
+;; This material is work in progress, more precisely at pre-Alpha quality as  ;;
+;; per Arm’s quality standards.                                               ;;
+;; In particular, this means that it would be premature to base any           ;;
+;; production tool development on this material.                              ;;
+;; However, any feedback, question, query and feature request would be most   ;;
+;; welcome; those can be sent to Arm’s Architecture Formal Team Lead          ;;
+;; Jade Alglave <jade.alglave@arm.com>, or by raising issues or PRs to the    ;;
+;; herdtools7 github repository.                                              ;;
+;;****************************************************************************;;
+
+(in-package "ASL")
+
+;; TODO: Document and add the stdlib proofs.
+
+(include-book "toplevel")
+(include-book "proofs/stdlib/top")
+(include-book "xdoc/save" :dir :system)
+(include-book "oslib/date" :dir :system)
+(defttag :manual-info)
+
+(value-triple (acl2::tshell-ensure))
+(defconsts (*herdtools-git-hash* state)
+  (b* (((mv ?ok lines state)
+        (acl2::tshell-call "git rev-parse HEAD")))
+    (mv (subseq (car lines) 0 8) state)))
+
+(defconsts (*acl2-git-hash* state)
+  (b* ((dir (acl2::include-book-dir :system state))
+       ((mv ?ok lines state)
+        (acl2::tshell-call (concatenate 'string
+                                        "cd " dir "; git rev-parse HEAD"))))
+    (mv (subseq (car lines) 0 8) state)))
+
+(defconsts (*manual-date* state) (oslib::date))
+
+
+(defxdoc acl2::top
+  :short "ACL2 ASL interpreter manual"
+  :long "<p>This manual was built on @(`(:raw *manual-date*)`) from Herdtools7 git
+version @(`(:raw *herdtools-git-hash*)`) and ACL2 git version @(`(:raw
+*acl2-git-hash*)`). See @(see asl) for a starting point.</p>")
+
+(xdoc::save "./manual" :error t)
